Composition/Dominant_Instances.thy
@@ -1,0 +1,13 @@
+theory Dominant_Instances
+  imports Dominant
+begin
+
+(*
+  do we need sups_pres ok_S?
+  i think it's ok if we require that,
+  it should be possible to prove
+*)
+
+(* sups_presI *)
+
+end
