Lifter/Auto_Lifter_Proofs_Examples.thy
@@ -51,6 +51,29 @@ lemma mrg2' :
 (schem_lift_S (SP NC (SP NB NA)) 
     (SP (SPRI (SO NA)) (SP (SPRI (SO NB)) (SPRI (SO NC))))) "
   unfolding schem_lift_defs schem_lift_S_defs
-by(fastforce intro: lifting_valid_noaxiom lifting_ortho_noaxiom)
+  by(fastforce intro: lifting_valid_noaxiom lifting_ortho_noaxiom)
+
+lemma mrg2'' :
+  "lifting_valid (schem_lift (SP NC (SP NB NA)) 
+    (SP (SPRI (SO NA)) (SP (SPRI (SO NB)) (SPRI (SO NC)))))
+(\<lambda> _ . ok_S) "
+  unfolding schem_lift_defs schem_lift_S_defs
+  apply(auto intro: lifting_valid_noaxiom lifting_ortho_noaxiom)
+  apply(rule lifting_valid.intro)
+  apply(rule merge_l_valid_weak.ax_g)
+    apply(auto intro: lifting_valid_noaxiom lifting_ortho_noaxiom)
+   apply(rule merge_l_valid_weak.intro)
+  apply(rule merge_l_ortho.ax_g_comm)
+    apply(auto intro: lifting_valid_noaxiom lifting_ortho_noaxiom)
+     apply(rule merge_l_ortho.intro)
+  apply(rule fst_l_snd_l_ortho.ax_g_comm)
+         apply(auto intro: lifting_valid_noaxiom lifting_ortho_noaxiom simp add: ok_S_defs)
+  apply(rule fst_l_snd_l_ortho.intro)
+         apply(auto intro: lifting_valid_noaxiom lifting_ortho_noaxiom simp add: ok_S_defs)
+               apply(rule fst_l_valid_base_ext.ax)
+               apply(rule fst_l_valid_base_ext.intro)
+               apply(rule prio_l_valid_base_ext.ax)
+               apply(rule prio_l_valid_base_ext.intro)
+         apply(auto intro: lifting_valid_noaxiom lifting_ortho_noaxiom simp add: ok_S_defs)
 
 end
